<?xml version="1.0" encoding="UTF-8"?>
<rdf:RDF
    xmlns:rdf="http://www.w3.org/1999/02/22-rdf-syntax-ns#"
    xmlns:skos="http://www.w3.org/2004/02/skos/core#">
    
    <skos:Concept rdf:about="#ResponseTime">
        <skos:prefLabel>response time</skos:prefLabel>
        <skos:definition>
            The time between sending a valid service request and receiving a response for that request from the service.
            Note that this term does not state if or how the effect caused by the network latency or transfer speed 
            between the request sender and the server should be calculated. For accurate measurements the effects caused
            by network access should be minimized by measuring at a network location connected to the service with
            minimal latency and high transfer speed. If this is not possible, the typical network delay and latency
            experienced at the measurement location should be estimated and extracted from the measured service 
            request times.
        </skos:definition>
    </skos:Concept>
    
    <skos:Concept rdf:about="#ServicePerformance">
        <skos:prefLabel>service performance</skos:prefLabel>
        <skos:definition>
            A measure of a service working as expected and in a timely fashion. Performance should be measured 
            ia a way that makes comparison possible between services providing the same functionality 
            and information content.
        </skos:definition>
    </skos:Concept>
    
    
    <skos:Concept rdf:about="#RequestResponsePerformance">
        <skos:prefLabel>request response performance</skos:prefLabel>
        <skos:broader rdf:resource="#ServicePerformance" />
        <skos:related rdf:resource="#ResponseTime" />
        <skos:definition>
            Method of evaluting the performance of the service by measuring it's response time for 
            particular requests. The lower the response time for a particular operation, 
            the more performant the service is seen. The assumption here is that repeated tests do not
            affect the response time considerably, and that the service or the network connection
            between the tester and the service has no other use at the time of measurement
            that would considerably influence the response time.
        </skos:definition>
    </skos:Concept>
    
    <skos:Concept rdf:about="#InitialResponsePerformance">
        <skos:prefLabel>initial response performance</skos:prefLabel>
        <skos:broader rdf:resource="#RequestResponsePerformance" />
        <skos:definition>
           Request response performance measuring the time between sending the request
           and receiving the first byte(s) of the response back. Different from
           #RequestResponsePerformance only in cases where there is a measurable difference
           in receiving the first byte(s) and the whole response.
        </skos:definition>
    </skos:Concept>
    
    <skos:Concept rdf:about="#MinimumRequestResponsePerformance">
        <skos:prefLabel>minimum request performance</skos:prefLabel>
        <skos:broader rdf:resource="#RequestResponsePerformance" />
        <skos:definition>
            The the upper limit for the request performance measured in milliseconds.
        </skos:definition>
    </skos:Concept>
    
    <skos:Concept rdf:about="#ContinuousAvailability">
        <skos:prefLabel>service availability</skos:prefLabel>
        <skos:related rdf:resource="#MinimumRequestResponsePerformance" />
        <skos:definition>
            The percentage of time within a period a month an online service has been generally accessible
            and operating above its minimum request performance for its intended users using its intended 
            network access methods. A measured metric value shall be calculated by measuring the service 
            access continously at least 10 times an hour.
        </skos:definition>
    </skos:Concept>
    
    <skos:Concept rdf:about="#AvailabilityMonthly">
        <skos:prefLabel>monthly service availability</skos:prefLabel>
        <skos:broader rdf:resource="#ContinuousAvailability" />
        <skos:definition>
            Service availability measured or estimated over a period of one month. Unless a specific month is referred to,
            this shall be interpreted as any given 30-day period of time.
        </skos:definition>
    </skos:Concept>
    
    <skos:Concept rdf:about="#AvailabilityDaily">
        <skos:prefLabel>daily service availability</skos:prefLabel>
        <skos:broader rdf:resource="#ContinuousAvailability" />
        <skos:definition>
            Service availability measured or estimated over a period of one day (24 hours). Unless a specific day is referred to,
            this shall be interpreted as any given 24-hour period of time.
        </skos:definition>
    </skos:Concept>
    
    <skos:Concept rdf:about="#RequestCapacity">
        <skos:prefLabel>request capacity</skos:prefLabel>
        <skos:related rdf:resource="#MinimumRequestResponsePerformance" />
        <skos:definition>
            The number of new valid requests that can be successfully executed by a service within a given period of time 
            while staying above the minimum request performance.
        </skos:definition>
    </skos:Concept>
 
    <skos:Concept rdf:about="#RequestCapacityPerSecond">
        <skos:prefLabel>request capacity in second</skos:prefLabel>
        <skos:broader rdf:resource="#RequestCapacity" />
        <skos:definition>
            The number of new valid requests that can be successfully executed within one second 
            while staying above the minimum request performance.
        </skos:definition>
    </skos:Concept>
    
</rdf:RDF>
